lambda2Gmu/Preservation.v
@@ -36,25 +36,6 @@ Proof.
       applys~ okt_typ. applys* wft_subst_tb.
 Qed.
 
-(* Lemma ok_subst_tb : forall Σ Z P E F, *)
-(*   ok (E & (withtyp Z) & F) -> *)
-(*   wft Σ E P -> *)
-(*   ok (E & map (subst_tb Z P) F). *)
-(* Proof. *)
-(*   introv O W. induction F using env_ind. *)
-(*   - rewrite map_empty. rewrite concat_empty_r in *. *)
-(*     inversions O. exfalso; apply* empty_push_inv. *)
-(*     apply eq_push_inv in H. destructs H. subst*. *)
-(*   - rewrite map_push. rewrite concat_assoc in *. *)
-
-(*     lets HPI: okt_push_inv O; destruct HPI; subst. *)
-(*     + lets (?&?): (okt_push_typ_inv O). *)
-(*       applys~ okt_sub. *)
-(*     + inversions H. *)
-(*       lets (?&?&?): (okt_push_var_inv O). *)
-(*       applys~ okt_typ. applys* wft_subst_tb. *)
-(* Qed. *)
-
 Lemma okt_strengthen_simple : forall Σ E F,
     okt Σ (E & F) -> okt Σ E.
   introv O.
@@ -469,195 +450,11 @@ Ltac crush_ihred_gen :=
     crush_ihred e
   end.
 
-(* TODO move these to Infrastructure *)
-Lemma fv_open_tt : forall x T1 T2 k,
-    x \notin fv_typ T1 ->
-    x \notin fv_typ T2 ->
-    x \notin fv_typ (open_tt_rec k T1 T2).
-  introv f1 f2.
-  unfold open_tt.
-  lets [Ho | Ho]: fv_open T2 T1 k; rewrite Ho; eauto.
-Qed.
-
-Lemma fv_open_te : forall e k x T,
-    x \notin fv_trm e ->
-    x \notin fv_typ T ->
-    x \notin fv_trm (open_te_rec k T e).
-  induction e using trm_ind'; introv efresh Tfresh;
-    try solve [
-          cbn in *; eauto
-        | cbn in *;
-          rewrite notin_union;
-          split*; apply* fv_open_tt
-        ].
-  - cbn. cbn in efresh.
-    apply notin_fold.
-    + intros T' Tin.
-      unfold open_typlist_rec in Tin.
-      lets Tin2: Tin.
-      apply List.in_map_iff in Tin2.
-      destruct Tin2 as [T'' [T'eq T''in]].
-      subst.
-      apply* fv_open_tt.
-    + apply* IHe.
-  - cbn in *.
-    apply notin_fold.
-    + intros cl clin.
-      apply List.in_map_iff in clin.
-      destruct clin as [[cl'A cl'T] [cl'eq cl'in]].
-      subst. cbn.
-
-      rewrite List.Forall_forall in *.
-      fold (clauseTerm (clause cl'A cl'T)).
-      apply* H.
-
-      cbn.
-      fold (clauseTerm (clause cl'A cl'T)).
-      apply* fv_fold_in_clause.
-    + apply* IHe.
-      apply* fv_fold_base_clause.
-Qed.
-
-Lemma fv_open_te_many : forall Ts e x,
-    (forall T, List.In T Ts -> x \notin fv_typ T) ->
-    x \notin fv_trm e ->
-    x \notin fv_trm (open_te_many Ts e).
-  induction Ts as [| Th Tts]; introv Tfresh efresh.
-  - cbn. trivial.
-  - cbn. apply IHTts.
-    + introv Tin. eauto with listin.
-    + unfold open_te.
-      apply fv_open_te; eauto with listin.
-Qed.
-
-Fixpoint subst_te_many (Xs : list var) (Us : list typ) (e : trm) :=
-  match (Xs, Us) with
-  (* | ((List.cons X Xt), (List.cons U Ut)) => subst_tt X U (subst_tt_many Xt Ut T) *)
-  | ((List.cons X Xt), (List.cons U Ut)) => subst_te_many Xt Ut (subst_te X U e)
-  | _ => e
-  end.
-
-Lemma subst_commutes_with_unrelated_opens_te : forall Xs e V Y,
-    (forall X, List.In X Xs -> X <> Y) ->
-    type V ->
-    subst_te Y V (open_te_many_var Xs e) =
-    (open_te_many_var Xs (subst_te Y V e)).
-  induction Xs as [| Xh Xt]; introv Hneq Htyp.
-  - cbn. eauto.
-  - cbn.
-    fold (open_te_many_var Xt (e open_te_var Xh)).
-    fold (open_te_many_var Xt (subst_te Y V e open_te_var Xh)).
-    rewrite* subst_te_open_te_var; eauto with listin.
-Qed.
-
-Lemma subst_intro_commutes_opens_te : forall Xs e Y V,
-    Y \notin fv_trm e ->
-    (forall X, List.In X Xs -> X <> Y) ->
-    type V ->
-    open_te_many_var Xs (open_te e V) =
-    subst_te Y V (open_te_many_var Xs (e open_te_var Y)).
-  induction Xs as [| Xh Xt]; introv Hfv Hneq Htyp.
-  - cbn. apply* subst_te_intro.
-  - cbn.
-    fold (open_te_many_var Xt (open_te e V open_te_var Xh)).
-    fold (open_te_many_var Xt ((e open_te_var Y) open_te_var Xh)).
-    rewrite* subst_commutes_with_unrelated_opens_te.
-    f_equal.
-    rewrite* <- subst_te_open_te_var.
-    + rewrite* <- subst_te_intro.
-    + apply* Hneq. cbn; eauto.
-    + eauto with listin.
-Qed.
-
-Lemma subst_te_intro_many : forall Xs e Us,
-    length Xs = length Us ->
-    DistinctList Xs ->
-    (forall X, List.In X Xs -> X \notin fv_trm e) ->
-    (forall X U, List.In X Xs -> List.In U Us -> X \notin fv_typ U) ->
-    (forall U, List.In U Us -> type U) ->
-    open_te_many Us e = subst_te_many Xs Us (open_te_many_var Xs e).
-  induction Xs as [| Xh Xt]; introv Hleneq Hdistinct HXfv HXUfv XUtyp.
-  - destruct Us.
-    + cbv. trivial.
-    + inversions Hleneq.
-  - destruct Us as [| Uh Ut].
-    + inversions Hleneq.
-    + cbn.
-      fold (open_te_many_var Xt (e open_te_var Xh)).
-      inversions Hdistinct.
-      rewrite IHXt; auto with listin.
-      * f_equal.
-        rewrite <- subst_intro_commutes_opens_te; eauto with listin.
-        introv Xin.
-        intro; subst. contradiction.
-      * introv Xin.
-        apply fv_open_te; eauto with listin.
-Qed.
-
-Lemma open_tt_many_closed : forall As T,
-    type T ->
-    open_tt_many As T = T.
-  induction As; introv Hcl.
-  - cbn. trivial.
-  - cbn. unfold open_tt.
-    rewrite* <- open_tt_rec_type.
-Qed.
-
-Lemma subst_tt_many_free : forall As Ts T,
-    (forall A, List.In A As -> A \notin fv_typ T) ->
-    T = subst_tt_many As Ts T.
-  induction As; introv Afresh.
-  - cbn. trivial.
-  - destruct Ts.
-    + cbn. trivial.
-    + cbn. rewrite <- IHAs.
-      * symmetry. apply subst_tt_fresh.
-        auto with listin.
-      * intros.
-        rewrite subst_tt_fresh;
-          auto with listin.
-Qed.
-
-Lemma subst_te_many_commutes_open : forall As Ts e x,
-    length As = length Ts ->
-    (forall A, List.In A As -> x <> A) ->
-    (subst_te_many As Ts e) open_ee_var x
-    =
-    subst_te_many As Ts (e open_ee_var x).
-  induction As as [| Ah Ats]; introv Hlen Afresh.
-  - cbn. auto.
-  - destruct Ts as [| Th Tts]; cbn in Hlen; try congruence.
-    cbn. fold (open_ee (subst_te_many Ats Tts (subst_te Ah Th e)) (trm_fvar x)).
-    rewrite IHAts; auto with listin.
-    f_equal.
-    apply subst_te_open_ee_var.
-Qed.
-
 Definition subst_tb_many (As : list var) (Ps : list typ) (b : bind) : bind :=
   match b with
   | bind_typ => bind_typ
   | bind_var T => bind_var (subst_tt_many As Ps T)
   end.
-
-Lemma env_map_ext_id : forall T (E : env T) (f : T -> T),
-    (forall x, f x = x) ->
-    map f E = E.
-  induction E using env_ind; introv fext;
-    autorewrite with rew_env_map; trivial.
-  - rewrite* IHE.
-    rewrite fext.
-    trivial.
-Qed.
-
-Lemma env_map_compose : forall A B C (E : env A) (f : A -> B) (g : B -> C) (h : A -> C),
-    (forall x, g (f x) = h x) ->
-    map g (map f E) = map h E.
-  induction E using env_ind; introv Hcomp;
-    autorewrite with rew_env_map; trivial.
-  - lets IH: IHE f g h.
-    rewrite IH; auto.
-    rewrite Hcomp. trivial.
-Qed.
 
 Lemma typing_through_subst_te_many : forall As Σ E F e T Ps,
     {Σ, E & (add_types empty As) & F} ⊢ e ∈ T ->
@@ -667,10 +464,7 @@ Lemma typing_through_subst_te_many : forall As Σ E F e T Ps,
     (forall A, List.In A As -> A # F) ->
     (forall A P, List.In A As -> List.In P Ps -> A \notin fv_typ P) ->
     DistinctList As ->
-    (* Z \notin fv_typ P -> (* theoretically this assumption should not be needed as it should arise from wft E P /\ okt E + Z (so Z is not in E and P is wft in E so it cannot have free Z), but we can shift this responsibility up *) *)
-    (* CT = (subst_tt_many As Ts T) -> *)
     {Σ, E & map (subst_tb_many As Ps) F} ⊢ (subst_te_many As Ps e) ∈  subst_tt_many As Ps T.
-  (* TODO the thm statement needs some fixes *)
   induction As as [| Ah Ats]; introv Htyp Hlen Pwft AE AF AP Adist.
   - cbn. unfold subst_tb_many. cbn.
     rewrite env_map_ext_id;
